Update ZKBOO completeness with random_tapes

code/ZKBoo.ec
@@ -5,11 +5,6 @@ require import Commitment.
 (** Ignore: This is now the preferred setup but is not yet the default **)
 pragma -oldip. pragma +implicits.
 
-(* TODO index into view *)
-(* TODO constuct random tape *)
-(* pred valid_view w1 w2 k1 k2 = forall j, w1 = phi_decomp *)
-op valid_view w = w /\ true.
-
 clone import Commitment as Commit with
   type message <- view.
 
@@ -19,7 +14,7 @@ type statement  = (circuit * int).
 type witness    = int.
 type message    = output * output * output * Commit.commitment * Commit.commitment * Commit.commitment.
 type challenge  = int.
-type response   = public_key * ((view * randomness) * (view * randomness)).
+type response   = public_key * (((random_tape * view) * randomness) * ((random_tape * view) * randomness)).
 
 axiom challenge_size (c : challenge) : 0 < c <= 3.
 
@@ -49,19 +44,27 @@ clone import SigmaProtocols as Sigma with
   qed.
 export Sigma.
 
+pred valid_view (view view2 : view) (c : circuit) (k1 k2 : random_tape) =
+  (forall i, 0 <= i /\ i + 1 < size view =>
+    (nth 0 view (i + 1)) = phi_decomp (nth (ADDC(0,0)) c i) i 1 view view2 k1 k2).
+
 module ZKBoo(Com : Protocol) : SProtocol = {
   var pk : public_key
   var r1, r2, r3 : randomness
   var w1, w2, w3 : view
+  var k1, k2, k3 : view
   proc gen() : statement * witness = {
     return (([], 0),0);
   }
   proc init(h : statement, w : witness) = {
-    var x1,x2,x3,y,c,c1,c2,c3,sk,y1,y2,y3;
+    var x1,x2,x3,y,c,c1,c2,c3,sk,y1,y2,y3,k1,k2,k3;
     (c, y) = h;
     (sk, pk) <$ Commit.dkey;
     (x1, x2, x3) = Phi.share(w);
-    (w1, w2, w3) = Phi.compute(c, [x1], [x2], [x3]);
+    k1 = [];
+    k2 = [];
+    k3 = [];
+    (k1, k2, k3, w1, w2, w3) = Phi.compute(c, [x1], [x2], [x3], k1, k2, k3);
     (c1, r1) = Com.commit(sk, w1);
     (c2, r2) = Com.commit(sk, w2);
     (c3, r3) = Com.commit(sk, w3);
@@ -75,12 +78,12 @@ module ZKBoo(Com : Protocol) : SProtocol = {
   proc response(h : statement, w : witness, m : message, e : challenge) = {
     var ret;
     if (e = 1) {
-      ret = ((w1, r1), (w2, r2));
+      ret = (((k1, w1), r1), ((k2, w2), r2));
     } else {
       if (e = 2) {
-        ret = ((w2, r2), (w3, r3));
+        ret = (((k2, w2), r2), ((k3, w3), r3));
       } else {
-        ret = ((w3, r3), (w1, r1));
+        ret = (((k3, w3), r3), ((k1, w1), r1));
       }
     }
     return (pk, ret);
@@ -92,53 +95,45 @@ module ZKBoo(Com : Protocol) : SProtocol = {
     return y = share;
   }
 
-  (* proc valid_view(w w' : view, k k' : random_tape) = { *)
-  (*   while (w <> []) { *)
-  (*     s = head w; *)
-  (*     s' = head w'; *)
-  (*     r = head k; *)
-  (*     r' = head k'; *)
-
-  (*     (* TODO *) *)
-
-  (*     w = behead w; *)
-  (*     w' = behead w'; *)
-  (*     k = behead k; *)
-  (*     k' = behead k'; *)
-  (*   } *)
-  (* } *)
-
   proc verify(h : statement, m : message, e : challenge, z : response) = {
     var c, pk, open, y1, y2, y3, c1, c2, c3, y, y', valid_com1, valid_com2;
     var valid_share1, valid_share2;
-    var w1', w2', w3', r1', r2', r3';
+    var w1', w2', w3', r1', r2', r3', o1, o2, k1', k2', k3';
     (pk, open) = z;
     (y1, y2, y3, c1, c2, c3) = m;
     (c, y) = h;
 
     if (e = 1) {
-      (w1', r1') = fst open;
-      (w2', r2') = snd open;
+      (o1, r1') = fst open;
+      (o2, r2') = snd open;
+      (k1', w1') = o1;
+      (k2', w2') = o2;
       valid_com1 = Commit.verify pk w1' c1 r1';
       valid_com2 = Commit.verify pk w2' c2 r2';
       valid_share1 = valid_output_share(y1, w1');
       valid_share2 = valid_output_share(y2, w2');
+      (* valid = valid_view w1' w2' c k1' k2'; *)
     } else {
       if (e = 2) {
-        (w2', r2') = fst open;
-        (w3', r3') = snd open;
+        (o1, r2') = fst open;
+        (o2, r3') = snd open;
+        (k2', w2') = o1;
+        (k3', w3') = o2;
         valid_com1 = Commit.verify pk w2' c2 r2';
         valid_com2 = Commit.verify pk w3' c3 r3';
         valid_share1 = valid_output_share(y2, w2');
         valid_share2 = valid_output_share(y3, w3');
+        (* valid = valid_view w2' w3' c k2' k3'; *)
       } else {
-        (w3', r3') = fst open;
-        (w1', r1') = snd open;
+        (o1, r3') = fst open;
+        (o2, r1') = snd open;
+        (k3', w3') = o1;
+        (k1', w1') = o2;
         valid_com1 = Commit.verify pk w3' c3 r3';
         valid_com2 = Commit.verify pk w1' c1 r1';
         valid_share1 = valid_output_share(y3, w3');
         valid_share2 = valid_output_share(y1, w1');
-
+        (* valid_view = valid_view w3' w1' c k3' k1'; *)
       }
     }
 
@@ -151,13 +146,17 @@ module ZKBoo(Com : Protocol) : SProtocol = {
   proc witness_extractor(h : statement, a : message,
                          e : challenge list, z : response list) = {
     var c, y, w1, w2, w3, r1, r2, r3, pk, open;
+    var o1, o2, o3, k1, k2, k3;
     (c, y) = h;
     (pk, open) = oget (onth z 0);
-    (w1, r1) = fst open;
+    (o1, r1) = fst open;
+    (k1, w1) = o1;
     (pk, open) = oget (onth z 1);
-    (w2, r2) = fst open;
+    (o2, r2) = fst open;
+    (k2, w2) = o2;
     (pk, open) = oget (onth z 2);
-    (w3, r3) = fst open;
+    (o3, r3) = fst open;
+    (k3, w3) = o3;
 
     return (oget (onth w1 0)) + (oget (onth w2 0)) + (oget (onth w3 0));
 
@@ -167,9 +166,10 @@ module ZKBoo(Com : Protocol) : SProtocol = {
     var c, y, views, sk, pk, a, z;
     var w1, w2, y1, y2, y3;
     var c1, c2, c3, r1, r2, r3;
+    var k1, k2;
     (c, y) = h;
     (views, y3) = Privacy.ideal(y, c, e);
-    (w1, w2) = views;
+    (k1, w1, k2, w2) = views;
     w3 <$ dlist dinput (size w1);
     y1 = Phi.output(w1);
     y2 = Phi.output(w2);
@@ -179,7 +179,7 @@ module ZKBoo(Com : Protocol) : SProtocol = {
     (c2, r2) = Com.commit(sk, w2);
     (c3, r3) = Com.commit(sk, w3);
     a = (y1, y2, y3, c1, c2, c3);
-    z = (pk, ((w1, r1), (w2, r2)));
+    z = (pk, (((k1, w1), r1), ((k2, w2), r2)));
 
     return (a, z);
   }
@@ -211,11 +211,14 @@ local module Intermediate = {
   }
 
   proc main(h : statement, w : witness, e : challenge) = {
-    var x1,x2,x3,sk,pk,y1,y2,y3,y';
+    var x1,x2,x3,sk,pk,y1,y2,y3,y',k1,k2,k3;
     var c,y,w1,w2,w3,valid_com1,valid_com2,valid_share1,valid_share2;
     (c, y) = h;
     (x1, x2, x3) = Phi.share(w);
-    (w1, w2, w3) = Phi.compute(c, [x1], [x2], [x3]);
+    k1 = [];
+    k2 = [];
+    k3 = [];
+    (k1, k2, k3, w1, w2, w3) = Phi.compute(c, [x1], [x2], [x3], k1, k2, k3);
     y1 = Phi.output(w1);
     y2 = Phi.output(w2);
     y3 = Phi.output(w3);
@@ -248,7 +251,7 @@ local module Intermediate = {
 }.
 
 local lemma inter_completeness h' w' e' &m:
-    R h' w' =>
+    R h' w' /\ valid_circuit h'.`1 =>
     Pr[Intermediate.main(h', w', e') @ &m : res] = 1%r.
 proof.
   rewrite /R /R_DL. rewrite pairS.
@@ -256,61 +259,50 @@ proof.
   byphoare(: (h = h' /\ w = w' /\ e = e') ==>)=>//; last first. smt().
   proc.
   case (e' = 1).
-    rcondt 8. auto. do ? call(:true); auto.
+    rcondt 11. auto. do ? call(:true); auto.
+    inline Intermediate.valid_output_share Phi.output Phi.reconstruct Phi.share.
+    auto.
     inline Intermediate.valid_output_share Phi.output Phi.reconstruct Phi.share.
     sp. wp.
     call commit_ll.
     call Com_correct.
     call Com_correct.
     auto.
-    call (compute_circuit_correct h'.`1 [w']).
-    auto; progress.
-    apply dinput_ll.
-    smt().
-    apply Commit.dkey_ll.
-    smt().
-    have : (result.`1, result.`2, result.`3) = result by smt().
-    rewrite /eval_circuit in H.
-    have Hlast := last_nth 0.
-    smt().
+    have Hcircuit := compute_circuit_correct h'.`1 [w'] [].
+    call Hcircuit.
+    auto; smt(dinput_ll Commit.dkey_ll nth_last size_ge0).
   case (e' = 2).
-    rcondf 8. auto. do ? call(:true); auto.
-    rcondt 8. auto. do ? call(:true); auto.
+    rcondf 11. auto. do ? call(:true); auto.
+    inline Intermediate.valid_output_share Phi.output Phi.reconstruct Phi.share.
+    auto.
+    rcondt 11. auto. do ? call(:true); auto.
+    inline Intermediate.valid_output_share Phi.output Phi.reconstruct Phi.share.
+    auto.
     inline Intermediate.valid_output_share Phi.output Phi.reconstruct Phi.share.
     sp. wp.
     call Com_correct.
     call Com_correct.
     call commit_ll.
     auto.
-    call (compute_circuit_correct h'.`1 [w']).
-    auto; progress.
-    apply dinput_ll.
-    smt().
-    apply Commit.dkey_ll.
-    smt().
-    have : (result.`1, result.`2, result.`3) = result by smt().
-    rewrite /eval_circuit in H.
-    have Hlast := last_nth 0.
+    have Hcircuit := compute_circuit_correct h'.`1 [w'] [].
+    call Hcircuit.
+    auto; smt(dinput_ll Commit.dkey_ll nth_last size_ge0).
   (* case (e' = 2) *)
-    smt().
-    rcondf 8. auto. do ? call(:true); auto.
-    rcondf 8. auto. do ? call(:true); auto.
+    rcondf 11. auto. do ? call(:true); auto.
+    inline Intermediate.valid_output_share Phi.output Phi.reconstruct Phi.share.
+    auto.
+    rcondf 11. auto. do ? call(:true); auto.
+    inline Intermediate.valid_output_share Phi.output Phi.reconstruct Phi.share.
+    auto.
     inline Intermediate.valid_output_share Phi.output Phi.reconstruct Phi.share.
     sp. wp.
     call Com_correct.
     call commit_ll.
     call Com_correct.
     auto.
-    call (compute_circuit_correct h'.`1 [w']).
-    auto; progress.
-    apply dinput_ll.
-    smt().
-    apply Commit.dkey_ll.
-    smt().
-    have : (result.`1, result.`2, result.`3) = result by smt().
-    rewrite /eval_circuit in H.
-    have Hlast := last_nth 0.
-    smt().
+    have Hcircuit := compute_circuit_correct h'.`1 [w'] [].
+    call Hcircuit.
+    auto; smt(dinput_ll Commit.dkey_ll nth_last size_ge0).
 qed.
 
 local equiv inter_equiv :
@@ -321,110 +313,136 @@ proof.
   inline ZKBoo(Com).init ZKBoo(Com).response ZKBoo(Com).verify.
   sp.
   case (e{1} = 1).
-  rcondt{1} 15. progress.
+  rcondt{1} 18. progress.
     auto; do ? call (:true); auto.
-  rcondt{2} 7. progress.
+    inline *. auto.
+  rcondt{2} 10. progress.
     auto; do ? call (:true); auto.
-  rcondt{1} 24. progress.
+    inline *. auto.
+  rcondt{1} 27. progress.
     auto; do ? call (:true); auto.
+    inline *. auto.
   inline Phi.reconstruct.
   inline ZKBoo(Com).valid_output_share Intermediate.valid_output_share.
   inline Intermediate.ComCorrectness.key_fixed.
-  swap{2} [11..12] 5.
-  swap{2} [15..18] 1.
-  swap{2} [3..5] 10.
-  swap{2} 2 1.
-  swap{1} 1 1.
-  auto.
-  sim.
-  auto.
-  call (:true); auto.
-  call (:true); auto.
-  call (:true); auto.
-  call (:true); auto.
-  call (:true); auto.
-  call (:true); auto.
-  call (:true). sim.
-  auto.
-  call (:true). sim.
-  skip; progress.
-  case (e{1} = 2).
-  rcondf{1} 15. progress.
-    auto; do ? call (:true); auto.
-  rcondt{1} 15. progress.
-    auto; do ? call (:true); auto.
-  rcondf{2} 7. progress.
-    auto; do ? call (:true); auto.
-  rcondt{2} 7. progress.
-    auto; do ? call (:true); auto.
-  rcondf{1} 24. progress.
-    auto; do ? call (:true); auto.
-  rcondt{1} 24. progress.
-    auto; do ? call (:true); auto.
-  inline Phi.reconstruct.
-  inline ZKBoo(Com).valid_output_share Intermediate.valid_output_share.
-  inline Intermediate.ComCorrectness.key_fixed.
-  auto. sim. auto.
-  swap{2} [12..13] 4.
+  swap{2} [6..8] 14.
+  swap{2} 6 - 5.
+  auto. sim.
   wp.
-  swap{2} [3..5] 10.
-  swap{2} 2 1.
-  swap{1} 1 1.
   call (:true); auto.
   call (:true); auto.
   call (:true); auto.
   call (:true); auto.
   call (:true); auto.
   call (:true); auto.
-  call (:true). sim.
-  auto.
-  call (:true). sim.
-  skip; progress.
+  call (:true); auto. sim.
+  call (:true); auto.
+
+  case (e{1} = 2).
+  rcondf{1} 18. progress.
+    auto; do ? call (:true); auto.
+    inline *; auto.
+  rcondt{1} 18. progress.
+    auto; do ? call (:true); auto.
+    inline *; auto.
+  rcondf{2} 10. progress.
+    auto; do ? call (:true); auto.
+    inline *; auto.
+  rcondt{2} 10. progress.
+    auto; do ? call (:true); auto.
+    inline *; auto.
+  rcondf{1} 27. progress.
+    auto; do ? call (:true); auto.
+    inline *; auto.
+  rcondt{1} 27. progress.
+    auto; do ? call (:true); auto.
+    inline *; auto.
+  inline Phi.reconstruct.
+  inline ZKBoo(Com).valid_output_share Intermediate.valid_output_share.
+  inline Intermediate.ComCorrectness.key_fixed.
+  swap{2} [6..8] 14.
+  swap{2} 6 - 5.
+  auto. sim.
+  wp.
+  call (:true); auto.
+  call (:true); auto.
+  call (:true); auto.
+  call (:true); auto.
+  call (:true); auto.
+  call (:true); auto.
+  call (:true); auto. sim.
+  call (:true); auto.
 
   (* case e = 3 *)
-  rcondf{1} 15. progress.
+  rcondf{1} 18. progress.
     auto; do ? call (:true); auto.
-  rcondf{1} 15. progress.
+    inline *; auto.
+  rcondf{1} 18. progress.
     auto; do ? call (:true); auto.
-  rcondf{2} 7. progress.
+    inline *; auto.
+  rcondf{2} 10. progress.
     auto; do ? call (:true); auto.
-  rcondf{2} 7. progress.
+    inline *; auto.
+  rcondf{2} 10. progress.
     auto; do ? call (:true); auto.
-  rcondf{1} 24. progress.
+    inline *; auto.
+  rcondf{1} 27. progress.
     auto; do ? call (:true); auto.
-  rcondf{1} 24. progress.
+    inline *; auto.
+  rcondf{1} 27. progress.
     auto; do ? call (:true); auto.
+    inline *; auto.
   inline Phi.reconstruct.
   inline ZKBoo(Com).valid_output_share Intermediate.valid_output_share.
   inline Intermediate.ComCorrectness.key_fixed.
-  auto. sim. auto.
-  swap{2} [11..12] 5. wp.
-  swap{2} [3..5] 10.
-  swap{2} 2 1.
-  swap{1} 1 1.
+  swap{2} [6..8] 14.
+  swap{2} 6 - 5.
+  auto. sim.
+  wp.
   call (:true); auto.
   call (:true); auto.
   call (:true); auto.
   call (:true); auto.
   call (:true); auto.
   call (:true); auto.
-  call (:true). sim.
-  auto.
-  call (:true). sim.
-  skip; progress.
+  call (:true); auto. sim.
+  call (:true); auto.
 qed.
 
 lemma zkboo_completeness h' w' e' &m:
-    R h' w' =>
+    R h' w' /\ valid_circuit h'.`1 =>
     Pr[Sigma.Completeness(ZKBoo(Com)).special(h', w', e') @ &m : res] = 1%r.
 proof.
   move=> rel.
   have -> : Pr[Completeness(ZKBoo(Com)).special(h', w', e') @ &m : res] =
             Pr[Intermediate.main(h', w', e') @ &m : res].
-  - byequiv inter_equiv=>//.
+  - byequiv inter_equiv=>/#.
   by have := inter_completeness h' w' e' &m rel.
 qed.
 
-lemma zkboo_shvzk
+lemma zkboo_shvzk h' a' z1 z2 z3 &m:
+    phoare[ZKBoo(Com).verify : h = h' /\ m = a' /\ e = 1 /\ z = z1 ==> res]= 1%r =>
+    phoare[ZKBoo(Com).verify : h = h' /\ m = a' /\ e = 2 /\ z = z2 ==> res]= 1%r =>
+    phoare[ZKBoo(Com).verify : h = h' /\ m = a' /\ e = 3 /\ z = z3 ==> res]= 1%r =>
+    Pr[Sigma.SpecialSoundness(ZKBoo(Com)).main(h', a', [1;2;3], [z1;z2;z3]) @ &m : res] = 1%r.
+proof.
+  move=> accept1 accept2 accept3.
+  byphoare(: h = h' /\ m = a' /\ c = [1;2;3] /\ z = [z1;z2;z3] ==>)=>//.
+  proc.
+  sp.
+  rcondt 1; auto.
+  rcondt 7. inline *. auto.
+  rcondt 13. inline *. auto.
+  rcondf 19. inline *. auto.
+  sp.
+  inline ZKBoo(Com).witness_extractor.
+  wp. call accept3.
+  wp. call accept2.
+  wp. call accept1.
+  skip; progress.
+  rewrite /R /R_DL.
+  (* need more information from res in accept(1|2|3) *)
+  (* namely, view reconstruct *)
+
 
 end section Protocol.
